Introduced new datatype update syntax:  D.(f := E) The old syntax, D[f := E], is still supported for a short while, but generates a warning about that syntax being deprecated. The new syntax also supports multiple updates:  D.(f := E0, g := E1, h := E2)

Source/Dafny/Cloner.cs
@@ -323,6 +323,10 @@ namespace Microsoft.Dafny
         var e = (SeqUpdateExpr)expr;
         return new SeqUpdateExpr(Tok(e.tok), CloneExpr(e.Seq), CloneExpr(e.Index), CloneExpr(e.Value));
 
+      } else if (expr is DatatypeUpdateExpr) {
+        var e = (DatatypeUpdateExpr)expr;
+        return new DatatypeUpdateExpr(Tok(e.tok), CloneExpr(e.Root), e.Updates.ConvertAll(t => Tuple.Create(Tok(t.Item1), t.Item2, CloneExpr(t.Item3))));
+
       } else if (expr is FunctionCallExpr) {
         var e = (FunctionCallExpr)expr;
         return new FunctionCallExpr(Tok(e.tok), e.Name, CloneExpr(e.Receiver), e.OpenParen == null ? null : Tok(e.OpenParen), e.Args.ConvertAll(CloneExpr));
